progress and preservation

lc_flat.v
@@ -1,20 +1,23 @@
 (* 
  * An encoding of the untyped lambda calculus with numbers.
  *
- * Authors: Arjun Guha <arjun@cs.brown.edu>
+ * Authors: 
+ *   Arjun Guha <arjun@cs.brown.edu>
+ *   Benjamin Lerner <blerner@cs.brown.edu>
  *)
 Require Import Coq.Arith.EqNat.
+Require Import Coq.Arith.Le.
+Require Import Coq.Arith.Lt.
 Require Import Coq.Structures.Orders.
 Require Import Coq.Arith.NatOrderedType.
 Require Import Coq.MSets.MSetList.
+Require Import Omega.
 Set Implicit Arguments.
 
 Module Type ATOM.
 
   Parameter atom : Set.
   Declare Module Atom_as_OT : UsualOrderedType with Definition t := atom.
-  Parameter atom_fresh_for_list :
-    forall (xs : list atom), exists x : atom, ~ List.In x xs.
 
 End ATOM.
 
@@ -27,7 +30,6 @@ Definition atom := Atom.atom. (* free variables *)
 Section Definitions.
 
 Inductive exp : Set :=
-  | exp_var  : atom -> exp
   | exp_bvar : nat -> exp (* bound variables as de Brujin indices *)
   | exp_abs  : exp -> exp
   | exp_app  : exp -> exp -> exp
@@ -43,7 +45,6 @@ Inductive exp : Set :=
 (* open_rec is the analogue of substitution for de Brujin indices.
   open_rec k u e replaces index k with u in e. *)
 Fixpoint open_rec (k : nat) (u : exp) (e : exp) { struct e } := match e with
-  | exp_var _     => e
   | exp_bvar n    => if beq_nat k n then u else e
   | exp_abs  e    => exp_abs (open_rec (S k) u e)
   | exp_app e1 e2 => exp_app (open_rec k u e1) (open_rec k u e2)
@@ -59,42 +60,25 @@ end.
 
 Definition open e u := open_rec 0 u e.
 
-
-Fixpoint subst (z : atom) (u : exp) (e : exp) := match e with
-  | exp_var y     => if Atom.Atom_as_OT.eq_dec z y then u else e
-  | exp_bvar _    => e
-  | exp_abs  e    => exp_abs (subst z u e)
-  | exp_app e1 e2 => exp_app (subst z u e1) (subst z u e2)
-  | exp_nat n     => e
-  | exp_succ e    => exp_succ (subst z u e)
-  | exp_bool b     => e
-  | exp_not e      => exp_not (subst z u e)
-  | exp_if e e1 e2 => exp_if (subst z u e) (subst z u e1) (subst z u e2)
-  | exp_err       => e
-  | exp_label x e => exp_label x (subst z u e)
-  | exp_break x e => exp_break x (subst z u e)
-end.
-
-Notation "e [ x / u ]" := (subst x u e) (at level 68).
-
 (* locally closed : all de Brujin indices are bound *)
-Inductive lc : exp -> Prop :=
-  | lc_var  : forall x, lc (exp_var x)
-  | lc_abs  : forall e L,
-    (forall x, (~ In x L) -> lc (open e (exp_var x)))
-    -> lc (exp_abs e)
-  | lc_app  : forall e1 e2, lc e1 -> lc e2 -> lc (exp_app e1 e2)
-  | lc_nat  : forall n, lc (exp_nat n)
-  | lc_succ : forall e, lc e -> lc (exp_succ e)
-  | lc_bool : forall b, lc (exp_bool b)
-  | lc_not  : forall e, lc e -> lc (exp_not e)
-  | lc_if   : forall e e1 e2, lc e -> lc e1 -> lc e2 -> lc (exp_if e e1 e2)
-  | lc_err  : lc exp_err
-  | lc_label : forall x e, lc e -> lc (exp_label x e)
-  | lc_break : forall x e, lc e -> lc (exp_break x e).
+Inductive lc' : nat -> exp -> Prop :=
+  | lc_bvar : forall k n, k < n -> lc' n (exp_bvar k)
+  | lc_abs  : forall n e,
+      lc' (S n) e -> lc' n (exp_abs e)
+  | lc_app  : forall n e1 e2, lc' n e1 -> lc' n e2 -> lc' n (exp_app e1 e2)
+  | lc_nat  : forall n x, lc' n (exp_nat x)
+  | lc_succ : forall n e, lc' n e -> lc' n (exp_succ e)
+  | lc_bool : forall n b, lc' n (exp_bool b)
+  | lc_not  : forall n e, lc' n e -> lc' n (exp_not e)
+  | lc_if   : forall n e e1 e2, 
+      lc' n e -> lc' n e1 -> lc' n e2 -> lc' n (exp_if e e1 e2)
+  | lc_err   : forall n, lc' n exp_err
+  | lc_label : forall n x e, lc' n e -> lc' n (exp_label x e)
+  | lc_break : forall n x e, lc' n e -> lc' n (exp_break x e).
+
+Definition lc e := lc' 0 e.
 
 Inductive val : exp -> Prop :=
-  | val_var : forall x, val (exp_var x)
   | val_abs : forall e, lc (exp_abs e) -> val (exp_abs e)
   | val_nat : forall n, val (exp_nat n)
   | val_bool : forall b, val (exp_bool b).
@@ -155,10 +139,10 @@ Inductive decompose1 : exp -> E -> exp -> Prop :=
       decompose1 (exp_app v e) (E_app_2 p E_hole) e
   | cxt1_succ : forall e,
       decompose1 (exp_succ e) (E_succ E_hole) e
-  | cxt1_not : forall e e',
-      decompose1 (exp_not e) (E_not E_hole) e'
-  | cxt1_if : forall e e1 e2 e',
-      decompose1 (exp_if e e1 e2) (E_if E_hole e1 e2) e'
+  | cxt1_not : forall e,
+      decompose1 (exp_not e) (E_not E_hole) e
+  | cxt1_if : forall e e1 e2,
+      decompose1 (exp_if e e1 e2) (E_if E_hole e1 e2) e
   | cxt1_break : forall x e,
       decompose1 (exp_break x e) (E_break x E_hole) e.
 
@@ -188,14 +172,10 @@ Inductive contract :  exp -> exp -> Prop :=
       val v -> contract (exp_app (exp_abs e) v) (open e v)
   | contract_err_app1 : forall n v,
       val v -> contract (exp_app (exp_nat n) v) exp_err
-  | contract_err_app2 : forall x v,
-      val v -> contract (exp_app (exp_var x) v) exp_err
   | contract_err_app3 : forall b v,
       val v -> contract (exp_app (exp_bool b) v) exp_err
   | contract_err_if1 : forall e e1 e2,
       contract (exp_if (exp_abs e) e1 e2) exp_err
-  | contract_err_if2 : forall x e1 e2,
-      contract (exp_if (exp_var x) e1 e2) exp_err
   | contract_err_if3 : forall n e1 e2,
       contract (exp_if (exp_nat n) e1 e2) exp_err
   | contract_label : forall x v,
@@ -223,52 +203,9 @@ Inductive step : exp -> exp -> Prop :=
 
 End Definitions.
 
-Hint Constructors decompose E val exp pot_redex exp val pot_redex lc contract
+Hint Constructors decompose E val exp pot_redex exp val pot_redex lc' contract
                   step decompose1.
-Hint Unfold open.
-
-Lemma open_rec_lc_core : forall e v i j u,
-  i <> j ->
-  open_rec j v e = open_rec i u (open_rec j v e) ->
-  e = open_rec i u e.
-Proof with eauto.
-  induction e; intros; simpl in *; try solve [ inversion H0; f_equal; eauto].
-  remember (beq_nat j n).
-  destruct b...
-  remember (beq_nat i n).
-  destruct b...
-  apply beq_nat_eq in Heqb.
-  apply beq_nat_eq in Heqb0.
-  contradiction H. clear H0. subst. auto.
-Qed.
-
-Lemma open_rec_lc : forall k u e,
-  lc e ->
-  e = open_rec k u e.
-Proof with auto.
-  intros.
-  generalize dependent k.
-  induction H...
-  simpl.
-  intros.
-  unfold open in *.
-  f_equal.
-  assert (exists x : atom, ~ In x L).
-    apply Atom.atom_fresh_for_list.
-  inversion H1.
-  apply open_rec_lc_core with (i := S k) (j := 0) (u := u) (v := exp_var x).
-  auto with arith.  
-  auto.  
-
-  intros. simpl. f_equal. auto. auto.
-  intros. simpl. f_equal. auto. auto.
-  intros. simpl. f_equal. auto. auto.
-  intros. simpl. f_equal. auto. auto.
-  intros. simpl. f_equal. auto. auto.
-  intros. simpl. f_equal. auto. auto.
-  intros. simpl. f_equal. auto. 
-Qed.
-
+Hint Unfold open lc.
 
 Lemma decompose_pot_redex : forall e E ae,
   decompose e E ae -> pot_redex ae.
@@ -293,29 +230,44 @@ Lemma decompose_lc : forall E e ae,
   lc ae.
 Proof. intros. induction H0; inversion H; eauto. Qed.
 
-Ltac solve_decomp := match goal with
-  | [ H1 : lc ?e,
+Lemma decompose1_lc : forall E e ae,
+  lc e ->
+  decompose1 e E ae ->
+  lc ae.
+Proof. intros. induction H0; try (inversion H; eauto). Qed.
+
+Ltac solve_decomp' := match goal with
+  | [ H1 : lc' 0 ?e,
       IHe : val ?e \/ 
             (exists E' : E, exists ae : exp, decompose ?e E' ae)
       |- val ?exp \/ (exists E0 : E, exists ae : exp, decompose ?exp E0 ae) ]
     => (destruct IHe; right; eauto; destruct_decomp e; eauto)
-  | _ => fail
+  | [ |- _] => fail "solve_decomp'"
+end.
+
+Lemma ZZ : 0 = 0. reflexivity. Qed.
+
+Ltac solve_decomp := match goal with
+  | [ IH : 0 = 0 -> _ |- _ ]
+    => (let Hidiot := fresh "x" in remember (IH ZZ) as Hidiot; solve_decomp')
+  | [ |- _ ] => fail "flasd"
 end.
 
 Lemma decomp : forall e,
   lc e -> val e \/ 
-          (* (exists e', exists x, e = exp_label x e') \/  *)
           (exists E, exists ae, decompose e E ae).
 Proof with eauto.
 intros.
-induction H; intros; try solve_decomp...
-(* exp_app *)
-destruct IHlc1; right...  destruct IHlc2...
+unfold lc in H.
+remember 0.
+induction H; intros; subst; try solve_decomp...
+inversion H.
+destruct IHlc'1. auto. right...  destruct IHlc'2. auto. eauto.
 destruct_decomp e2. exists (E_app_2 H1 E)...
-destruct_decomp e1. exists (E_app_1 E e2)...
+destruct_decomp e1. right. exists (E_app_1 E e2)...
 Qed.
 
-Hint Resolve decompose_lc.
+Hint Resolve decompose_lc decompose1_lc.
 
 Lemma progress : forall e,
   lc e ->
@@ -335,8 +287,8 @@ inversion H0; subst;
 Qed.
 
 Ltac solve_lc_plug := match goal with
-  | [ IHdecompose : lc ?e -> lc (plug ?e' ?E),
-      H : lc ?e
+  | [ IHdecompose : lc' 0 ?e -> lc' 0 (plug ?e' ?E),
+      H : lc' 0 ?e
       |- context [plug ?e' ?E] ]
     => (apply IHdecompose in H; auto)
 end.
@@ -348,41 +300,74 @@ Lemma lc_plug : forall E ae e e',
   lc (plug e' E).
 Proof.
 intros.
-induction H1; first [ inversion H; subst; simpl; solve_lc_plug | auto ].
+induction H1; first [ inversion H; subst; simpl; unfold lc in *; solve_lc_plug | auto ].
 Qed.
 
 Hint Resolve lc_plug.
 
 Lemma lc_val : forall v,
-  val v -> lc v.
+  val v -> lc' 0 v.
 Proof with auto.
 intros. inversion H... Qed.
 
 Lemma lc_active : forall e,
   pot_redex e -> lc e.
-Proof. intros. inversion H; auto using lc_val. Qed.
+Proof. intros. unfold lc. inversion H; auto using lc_val. Qed.
 
 Hint Resolve lc_active.
 
-Lemma lc_open : forall k e u x,
-  lc (open_rec k (exp_var x) e) ->
-  lc u ->
-  lc (open_rec k u e).
+Lemma lc_ascend : forall k k' e, k' >= k -> lc' k e -> lc' k' e.
 Proof with auto.
 intros.
-generalize dependent k. generalize dependent u.
-induction e; intros; simpl...
-simpl in H.
-destruct (beq_nat k n)...
-simpl in H.
-inversion H; subst.
-eapply lc_abs with L.
-intros.
-unfold open. 
-unfold open in H2.
-assert (E := H2 x0 H1).
-admit.
+generalize dependent k'.
+induction H0...
+intros. apply lc_bvar. omega.
+intros. apply lc_abs. apply IHlc'. omega.
+Qed.
 
+Lemma lc_open : forall k e u,
+  lc' (S k) e ->
+  lc' 0 u ->
+  lc' k (open_rec k u e).
+Proof with auto.
+intros.
+generalize dependent k.
+induction e; intros.
+simpl...
+simpl. 
+assert (k >= n \/ k < n). apply le_or_lt.
+destruct H1.
+assert ({ k = n } + { k <> n }). decide equality.
+destruct H2.
+assert (beq_nat k n = true). rewrite -> beq_nat_true_iff...
+rewrite -> H2.  assert (k >= 0). omega.
+  apply lc_ascend with (k := 0) (k' := k)...
+assert (beq_nat k n = false).  rewrite -> beq_nat_false_iff...
+rewrite -> H2.
+assert (n < k). omega. auto...
+(* k < n *)
+assert (beq_nat k n = false).  rewrite -> beq_nat_false_iff... omega.
+rewrite -> H2. apply lc_bvar.
+clear H2.
+inversion H; subst.
+assert False. omega.
+inversion H2.
+(* abs *) 
+simpl.
+apply lc_abs.
+inversion H; subst.
+apply (IHe (S k) H3).
+(* app *)
+simpl; inversion H; subst;  eauto.
+simpl; inversion H; subst;  eauto.
+simpl; inversion H; subst;  eauto.
+simpl; inversion H; subst;  eauto.
+simpl; inversion H; subst;  eauto.
+simpl; inversion H; subst;  eauto.
+simpl; inversion H; subst;  eauto.
+simpl; inversion H; subst;  eauto.
+simpl; inversion H; subst;  eauto.
+Qed.
 
 Lemma lc_contract : forall ae e,
   lc ae ->
@@ -395,13 +380,19 @@ simpl. destruct e; auto.
 simpl. destruct e; auto.
 inversion H...
 inversion H...
+(* app *)
+unfold lc in *.
 inversion H; subst.
 unfold open.
-inversion H3; subst.
-unfold open in *.
-
-
-Admitted.
+inversion H4; subst.
+apply lc_open. exact H3. exact H5.
+(* break *)
+apply lc_val...
+(* break *)
+apply decompose1_lc with (E := E0) (e := e)...
+inversion H; inversion H2; subst...
+inversion H...
+Qed.
 
 Lemma preservation : forall e1 e2,
   lc e1 ->
@@ -409,6 +400,7 @@ Lemma preservation : forall e1 e2,
   lc e2.
 Proof with auto.
 intros.
+unfold lc in *.
 destruct H0. auto.
 assert (pot_redex ae). apply decompose_pot_redex with (e := e) (E := E0)...
 apply lc_active in H3.
